reformat paragraphs to 78 on the line

plugins/vdm2isa/src/main/resources/RecursiveVDM.thy
@@ -7,51 +7,57 @@ begin
 
 (**************************************************************************************************)
 section \<open>Introduction\label{sec:Intro}\<close>
+text \<open>This paper describes a translation strategy for a variety of recursive
+definitions from VDM to Isabelle/HOL. The strategy takes into account the
+differences in how termination and well-foundedness are represented in both
+formalisms.
 
-text \<open>This paper describes a translation strategy for a variety of recursive 
-definitions from VDM to Isabelle/HOL. The strategy takes 
-into account the differences in how termination and well-foundedness 
-are represented in both formalisms. 
+Beyond overcoming technical practicalities, which we discuss, a major
+objective is to create translation strategy templates. These templates must
+cover a wide variety of VDM recursive definitions, as well as having their
+proof obligations being highly automated. The result is an extension to the
+VDM to Isabelle/HOL translation strategy and implementation as a plugin to
+VDMJ~@{cite Battle09} and extension to VDM-VSCode @{cite AdvancedVSCodePaper}.
 
-Beyond overcoming technical practicalities, which we discuss, a major objective is to create
-translation strategy templates. These templates must cover a wide variety of VDM 
-recursive definitions, as well as having their proof obligations being highly automated.
-The result is an extension to the VDM to Isabelle/HOL translation strategy and implementation 
-as a plugin to VDMJ~@{cite Battle09} and extension to VDM-VSCode @{cite AdvancedVSCodePaper}.
+Isabelle uses literate programming, where formal specification, proofs and
+documentation are all within the same environment. We omit proofs scripts
+below; the full VDM and Isabelle sources and proofs can be found at the VDM
+toolkit repository at
+\<^verbatim>\<open>./plugins/vdm2isa/src/main/resources/RecursiveVDM.*\<close>\<^footnote>\<open>in~\<^url>\<open>https://github.com/leouk/VDM_Toolkit\<close>\<close>.
 
-Isabelle uses literate programming, where formal specification, proofs and documentation are
-all within the same environment. We omit proofs scripts below; the full VDM and Isabelle sources 
-and proofs can be found at the VDM toolkit repository at
- \<^verbatim>\<open>./plugins/vdm2isa/src/main/resources/RecursiveVDM.*\<close>\<^footnote>\<open>in~\<^url>\<open>https://github.com/leouk/VDM_Toolkit\<close>\<close>.
-
-In the next section, we present background on VDM and Isabelle recursion and measure relations.
-In Section~\ref{sec:VDMTypes}, we briefly discuss VDM basic types translation and their
-consequence for recursion. Next, Section~\ref{sec:Recursion} describes how both VDM
-and Isabelle recursive definitions work and how they differ. Our translation strategy
-is then presented in Section~\ref{sec:Strategy} for basic types, sets, maps, and 
-complex recursive patterns. Finally, we conclude in Section~\ref{sec:Conclusion}. 
-\<close>
+In the next section, we present background on VDM and Isabelle recursion and
+measure relations. In Section~\ref{sec:VDMTypes}, we briefly discuss VDM basic
+types translation and their consequence for recursion. Next,
+Section~\ref{sec:Recursion} describes how both VDM and Isabelle recursive
+definitions work and how they differ. Our translation strategy is then
+presented in Section~\ref{sec:Strategy} for basic types, sets, maps, and
+complex recursive patterns. Finally, we conclude in
+Section~\ref{sec:Conclusion}. \<close>
 
 (**************************************************************************************************)
 section \<open>Background\label{sec:Background}\<close> 
 
-text \<open>Our VDM to Isabelle/HOL translator caters for a wide range of the VDM AST. It copes with all kinds 
-of expressions, a variety of patterns, almost all types, imports and exports, functions and specifications,
-traces, and some of state and operations @{cite NimFull and AdvancedVSCodePaper}. 
-Even though not all kinds of VDM patterns are allowed,
-the translator copes with most, and where it does not, a corresponding equivalent is possible.
+text \<open>Our VDM to Isabelle/HOL translator caters for a wide range of the VDM
+AST. It copes with all kinds of expressions, a variety of patterns, almost all
+types, imports and exports, functions and specifications, traces, and some of
+state and operations @{cite NimFull and AdvancedVSCodePaper}. Even though not
+all kinds of VDM patterns are allowed, the translator copes with most, and
+where it does not, a corresponding equivalent is possible.
 
-One particular area we want to extend translation is over recursively defined functions. 
-VDM requires the user to define a measure function to justify why recursion will 
-terminate. It then generates proof obligations to ensure totality and termination. 
+One particular area we want to extend translation is over recursively defined
+functions. VDM requires the user to define a measure function to justify why
+recursion will terminate. It then generates proof obligations to ensure
+totality and termination.
 
-Finally, our translation strategy follows the size-change termination (SCT) proof 
-strategy described in @{cite SCT_POPL and SCNP_POPL}. In particular, its SCP (polynomial) and SCNP (non-polynomial)
-subclasses of recursive definitions within the SCT, which permits efficient termination checking. 
-Effectively, if every infinite computation would give rise to an infinitely decreasing value sequence 
-(according to the size-change principle), then no infinite computation is possible. Termination problems in 
-this class have a global ranking function of a certain form, which can be found using SAT solving, hence 
-increasing automation.
+Finally, our translation strategy follows the size-change termination (SCT)
+proof strategy described in @{cite SCT_POPL and SCNP_POPL}. In particular, its
+SCP (polynomial) and SCNP (non-polynomial) subclasses of recursive definitions
+within the SCT, which permits efficient termination checking. Effectively, if
+every infinite computation would give rise to an infinitely decreasing value
+sequence (according to the size-change principle), then no infinite
+computation is possible. Termination problems in this class have a global
+ranking function of a certain form, which can be found using SAT solving,
+hence increasing automation.
 
 \<^bold>\<open>ANYTHING ELSE? Related work?\<close>
 \<close>
@@ -59,39 +65,47 @@ increasing automation.
 (**************************************************************************************************)
 section \<open>VDM basic types in Isabelle\label{sec:VDMTypes}\<close>
 
-text \<open>Isabelle represents natural numbers (\<^typ>\<open>\<nat>\<close>) as a (data) type with two constructors (\<^term>\<open>0::\<nat>\<close> and \<^term>\<open>Suc n\<close>), 
-  where all numbers are projections over such constructions (\<^emph>\<open>e.g.\<close>~@{lemma "2 = (Suc (Suc 0))" by simp}).   
-  Isabelle integers (\<^typ>\<open>\<int>\<close>) are defined as a quotient type involving two natural numbers. Isabelle quotient types are 
-  injections into a constructively defined type. Like with integers, other
-  Isabelle numeric types (\<^emph>\<open>e.g.,\<close>~rationals \<^typ>\<open>\<rat>\<close>, reals \<^typ>\<open>\<real>\<close>, \<^emph>\<open>etc\<close>.) are defined in terms of some
-  involved natural number construction. Type conversions (or coercions) are then defined to allow users to jump
-  between type spaces. Nevertheless, Isabelle has no implicit type widening rule for \<^typ>\<open>\<nat>\<close>; instead, it takes 
-  conventions like @{lemma[show_types] \<open>(0 - x::\<nat>) = 0\<close> by simp}. For expressions involving 
-a mixutre of \<^typ>\<open>\<int>\<close> and \<^typ>\<open>\<nat>\<close> typed terms, explicit user-defined
-  type coercions might be needed (\<^emph>\<open>e.g.,\<close>~@{lemma[show_types] \<open>(2::\<nat>) - (3::\<int>) = -1\<close> by simp}).
+text \<open>Isabelle represents natural numbers (\<^typ>\<open>\<nat>\<close>) as a (data) type with
+two constructors (\<^term>\<open>0::\<nat>\<close> and \<^term>\<open>Suc n\<close>), where all numbers are
+projections over such constructions (\<^emph>\<open>e.g.\<close>~@{lemma "2 = (Suc (Suc 0))" by
+simp}). Isabelle integers (\<^typ>\<open>\<int>\<close>) are defined as a quotient type
+involving two natural numbers. Isabelle quotient types are injections into a
+constructively defined type. Like with integers, other Isabelle numeric types
+(\<^emph>\<open>e.g.,\<close>~rationals \<^typ>\<open>\<rat>\<close>, reals \<^typ>\<open>\<real>\<close>, \<^emph>\<open>etc\<close>.) are defined in
+terms of some involved natural number construction. Type conversions (or
+coercions) are then defined to allow users to jump between type spaces.
+Nevertheless, Isabelle has no implicit type widening rule for \<^typ>\<open>\<nat>\<close>;
+instead, it takes conventions like @{lemma[show_types] \<open>(0 - x::\<nat>) = 0\<close> by
+simp}. For expressions involving a mixutre of \<^typ>\<open>\<int>\<close> and \<^typ>\<open>\<nat>\<close> typed
+terms, explicit user-defined type coercions might be needed
+(\<^emph>\<open>e.g.,\<close>~@{lemma[show_types] \<open>(2::\<nat>) - (3::\<int>) = -1\<close> by simp}).
  
-   VDM expressions with basic-typed (\<^bold>\<open>nat\<close>, \<^bold>\<open>int\<close>) variables have specific type widening rules.
-  For example, even if both variables are \<^bold>\<open>nat\<close>, the result might be \<^bold>\<open>int\<close>. 
-(\<^emph>\<open>e.g.,\<close>~in VDM, \<^verbatim>\<open>0 - x:nat = -x:int\<close>). Therefore, our translation 
-  strategy considers VDM \<^bold>\<open>nat\<close> as the Isabelle type \<^typ>\<open>VDMNat\<close>, which is just a type synonym for \<^typ>\<open>\<int>\<close>. This 
-  simplifies the translation process to Isabelle, such that no type coercions are necessary to encode all VDM type widenning rules. 
-  On the other hand, this design decision means encoding of recursive functions over \<^bold>\<open>nat\<close> to be more complicated 
-  than expected, given VDM's \<^bold>\<open>nat\<close> is represented as Isabelle's \<^typ>\<open>\<int>\<close>.
+ VDM expressions with basic-typed (\<^bold>\<open>nat\<close>, \<^bold>\<open>int\<close>) variables have specific
+ type widening rules. For example, even if both variables are \<^bold>\<open>nat\<close>, the
+ result might be \<^bold>\<open>int\<close>. (\<^emph>\<open>e.g.,\<close>~in VDM, \<^verbatim>\<open>0 - x:nat = -x:int\<close>). Therefore,
+ our translation strategy considers VDM \<^bold>\<open>nat\<close> as the Isabelle type
+ \<^typ>\<open>VDMNat\<close>, which is just a type synonym for \<^typ>\<open>\<int>\<close>. This simplifies
+ the translation process to Isabelle, such that no type coercions are
+ necessary to encode all VDM type widenning rules. On the other hand, this
+ design decision means encoding of recursive functions over \<^bold>\<open>nat\<close> to be more
+ complicated than expected, given VDM's \<^bold>\<open>nat\<close> is represented as Isabelle's
+ \<^typ>\<open>\<int>\<close>.
 
-  Despite this design decision over basic types and their consequences, recursion
-over VDM \<^bold>\<open>int\<close>, sets or maps will still be involved. That is because these types 
-are not constructively defined in Isabelle.\<close>
+  Despite this design decision over basic types and their consequences,
+  recursion over VDM \<^bold>\<open>int\<close>, sets or maps will still be involved. That is
+  because these types are not constructively defined in Isabelle.\<close>
 
 (**************************************************************************************************)
 section \<open>Recursion in VDM and in Isabelle\label{sec:Recursion}\<close>
 
-text \<open>An important aspect of every recursive definition
-is an argument that justifies its termination. Otherwise, the recursion might go on 
-in an infinite loop. In VDM, this is defined using a recursive measure:~it has the same input type signature as
-the recursive definition, and returns a \<^bold>\<open>nat\<close>, which \<^bold>\<open>must\<close> monotonically decrease 
-at each recursive call, eventually reaching zero. This is how termination of recursive definitions 
-are justified in VDM. A simple example of a VDM recursive definition is one for calculating 
-the factorial of a given natural number
+text \<open>An important aspect of every recursive definition is an argument that
+justifies its termination. Otherwise, the recursion might go on in an infinite
+loop. In VDM, this is defined using a recursive measure:~it has the same input
+type signature as the recursive definition, and returns a \<^bold>\<open>nat\<close>, which
+\<^bold>\<open>must\<close> monotonically decrease at each recursive call, eventually reaching
+zero. This is how termination of recursive definitions are justified in VDM. A
+simple example of a VDM recursive definition is one for calculating the
+factorial of a given natural number
 %
 \begin{vdmsl}[frame=none,basicstyle=\ttfamily\scriptsize]
    fact: nat -> nat 
@@ -101,13 +115,13 @@ the factorial of a given natural number
 %   -- For the measure below, VDMJ produces a measure function as: 
 %   -- measure_fact: nat -> nat
 %   -- measure_fact(n) == n
-\noindent The \<^verbatim>\<open>fact\<close> recursive measure uses the \<^verbatim>\<open>n\<close> input itself as its result. 
-This works because the only recursive call is made with a decreasing value of \<^verbatim>\<open>n\<close>, 
-until it reaches \<^verbatim>\<open>0\<close> and terminates. VDMJ generates 
-three proof obligations for the definition above.
-They are trivial to discharge in Isabelle given the measure definition expanded is just 
+\noindent The \<^verbatim>\<open>fact\<close> recursive measure uses the \<^verbatim>\<open>n\<close> input itself as its
+result. This works because the only recursive call is made with a decreasing
+value of \<^verbatim>\<open>n\<close>, until it reaches \<^verbatim>\<open>0\<close> and terminates. VDMJ generates three
+proof obligations for the definition above. They are trivial to discharge in
+Isabelle given the measure definition expanded is just 
 @{lemma \<open>(\<forall> n::\<nat> . \<not> n = 0 \<longrightarrow> n - 1 \<ge> 0)\<close> by simp} and 
-@{lemma \<open>(\<forall> n::\<nat> . \<not> n = 0 \<longrightarrow> n > n - 1)\<close> by simp}. 
+@{lemma \<open>(\<forall> n::\<nat> . \<not> n = 0 \<longrightarrow> n > n - 1)\<close> by simp}.
 %
 \begin{vdmsl}[frame=none,basicstyle=\ttfamily\scriptsize]
 Proof Obligation 1: (Unproved) fact; measure_fact: total function obligation 
@@ -119,215 +133,234 @@ Proof Obligation 2: (Unproved) fact: subtype obligation
 Proof Obligation 3: (Unproved) fact: recursive function obligation 
 (forall n:nat & (not (n=0) => measure_fact(n) > measure_fact((n-1))))
 \end{vdmsl} 
-
+%
 %Remove?
-Moreover, even though measures over recursive type structures are impossible to define in VDM, they are 
-easily described in Isabelle. For example, it is not possible to write a measure in VDM  
-over a recursive record defining a linked list, such as \<^verbatim>\<open>R :: v: nat n: R\<close>. 
-This is automatically generated for our representation of VDM records in Isabelle as a datatype.
-Other complex recursive patterns are hard/impossible to represent in VDM (see Section~\ref{subsec:Complex}).   
+Moreover, even though measures over recursive type structures are impossible
+to define in VDM, they are easily described in Isabelle. For example, it is
+not possible to write a measure in VDM over a recursive record defining a
+linked list, such as \<^verbatim>\<open>R :: v: nat n: R\<close>. This is automatically generated for
+our representation of VDM records in Isabelle as a datatype. Other complex
+recursive patterns are hard/impossible to represent in VDM (see
+Section~\ref{subsec:Complex}).
   
-In Isabelle, recursive definitions can be provided through primitive recursion over inputs that are 
-constructively defined, or more general function definitions that produces proof obligations. 
-The former insists on definition for each type constructor and only provides simplification rules; whereas
-the latter allow for more sophisticated input patterns and provides simplification, elimination and 
-induction rules, as well as partial function considerations. For the purposes of this paper, we only 
-consider function definitions. Readers can find more about these differences in~@{cite IsaFunctionPackage}. 
+In Isabelle, recursive definitions can be provided through primitive recursion
+over inputs that are constructively defined, or more general function
+definitions that produces proof obligations. The former insists on definition
+for each type constructor and only provides simplification rules; whereas the
+latter allow for more sophisticated input patterns and provides
+simplification, elimination and induction rules, as well as partial function
+considerations. For the purposes of this paper, we only consider function
+definitions. Readers can find more about these differences in~@{cite
+IsaFunctionPackage}.
 
-Isabelle recursive functions requires a proof obligation that parameters represent a constructive and 
-compatible pattern, and that recursive calls terminate. Constructive patterns relates to all constructors 
-in data type being used in the recursion inputs (\<^emph>\<open>e.g.,\<close>~one equation for each of the constructors of \<^typ>\<open>\<nat>\<close>, 
-hence one involving \<^term>\<open>0::\<nat>\<close> and another involving \<^term>\<open>Suc n\<close>). Compatible patterns relates to multiple ways 
-patterns can be constructed will boil down to the pattern completeness cases (\<^emph>\<open>e.g.,\<close>~\<^term>\<open>n + 2::\<nat>\<close> being 
-simply multiple calls over defined constructors like \<^term>\<open>Suc (Suc n)\<close>). This is important to ensure that recursion 
-is well structured (\<^emph>\<open>i.e.,\<close>~recursive calls will not get stuck because some constructs are not available). 
-For example, if you miss the \<^term>\<open>0::\<nat>\<close> case, eventually the \<^term>\<open>Suc n\<close> case will reach zero and fail, as no patterns for zero exist. 
-The proof obligation for termination establishes that the recursion is well-founded. This has to be proved whenever 
-properties of the defined function are meant to be total. 
+Isabelle recursive functions requires a proof obligation that parameters
+represent a constructive and compatible pattern, and that recursive calls
+terminate. Constructive patterns relates to all constructors in data type
+being used in the recursion inputs (\<^emph>\<open>e.g.,\<close>~one equation for each of the
+constructors of \<^typ>\<open>\<nat>\<close>, hence one involving \<^term>\<open>0::\<nat>\<close> and another
+involving \<^term>\<open>Suc n\<close>). Compatible patterns relates to multiple ways
+patterns can be constructed will boil down to the pattern completeness cases
+(\<^emph>\<open>e.g.,\<close>~\<^term>\<open>n + 2::\<nat>\<close> being simply multiple calls over defined
+constructors like \<^term>\<open>Suc (Suc n)\<close>). This is important to ensure that
+recursion is well structured (\<^emph>\<open>i.e.,\<close>~recursive calls will not get stuck
+because some constructs are not available). For example, if you miss the
+\<^term>\<open>0::\<nat>\<close> case, eventually the \<^term>\<open>Suc n\<close> case will reach zero and
+fail, as no patterns for zero exist. The proof obligation for termination
+establishes that the recursion is well-founded. This has to be proved whenever
+properties of the defined function are meant to be total.
 
-Isabelle function definitions can be given with either \<^term>\<open>fun\<close> or \<^term>\<open>function\<close> syntax. The
-former attempts to automatically prove the pattern constructive and compatible proofs and 
-finds a measure for the termination proof obligation. The latter requires the user to do 
-these proofs manually by providing a measure relation. It is better suited for cases 
-where \<^term>\<open>fun\<close> declarations fail, which usually involve complex or ill-defined recursion. 
+Isabelle function definitions can be given with either \<^term>\<open>fun\<close> or
+\<^term>\<open>function\<close> syntax. The former attempts to automatically prove the
+pattern constructive and compatible proofs and finds a measure for the
+termination proof obligation. The latter requires the user to do these proofs
+manually by providing a measure relation. It is better suited for cases where
+\<^term>\<open>fun\<close> declarations fail, which usually involve complex or ill-defined
+recursion.
 
-The termination relation must be well-founded, which means have a
-well-ordered induction principle over a partially ordered relation defined as\<^footnote>\<open>For 
-details on what well-ordered induction means see theory \<^verbatim>\<open>Wellfounded.thy\<close> within Isabelle's distribution.\<close>
-@{thm[display,show_types] wf_def}. 
-A definition that Isabelle discovers all three proofs is\<close>
-(*
-find_theorems name:wellorder
-print_locale! wellorder *)
+The termination relation must be well-founded, which means have a well-ordered
+induction principle over a partially ordered relation defined as\<^footnote>\<open>For details
+on what well-ordered induction means see theory \<^verbatim>\<open>Wellfounded.thy\<close> within
+Isabelle's distribution.\<close> @{thm[display,show_types] wf_def}. A definition that
+Isabelle discovers all three proofs is\<close>
+(* find_theorems name:wellorder print_locale! wellorder *)
 fun fact' :: \<open>\<nat> \<Rightarrow> \<nat>\<close> where \<open>fact' n = (if n = 0 then 1 else n * (fact' (n - 1)))\<close> 
 
-text \<open>This definition is quite similar in VDM. 
-Nevertheless, VDM basic types widening rules 
-necessitated we translate them to \<^typ>\<open>VDMNat\<close>. 
-The same version of \<^term>\<open>fact\<close> defined for \<^typ>\<open>\<int>\<close> will fail with 
-the error that ``\<^emph>\<open>Could not find lexicographic termination order\<close>''. That is, 
-Isabelle manages to discharge the pattern proofs, but not the termination one. 
-This is because the user must provide a projection relation from the \<^typ>\<open>\<int>\<close> 
+text \<open>This definition is quite similar in VDM. Nevertheless, VDM basic types
+widening rules necessitated we translate them to \<^typ>\<open>VDMNat\<close>. The same
+version of \<^term>\<open>fact\<close> defined for \<^typ>\<open>\<int>\<close> will fail with the error that
+``\<^emph>\<open>Could not find lexicographic termination order\<close>''. That is, Isabelle
+manages to discharge the pattern proofs, but not the termination one. This is
+because the user must provide a projection relation from the \<^typ>\<open>\<int>\<close>
 quotient type back into the constructive type \<^typ>\<open>\<nat>\<close>.
 
-Even if we could avoid this translation technicality, 
-the same problem would occur for recursion over non constructive types, 
-such as sets or maps. They require recursion over finite sets, which are
-defined inductively.
-The only easy recursive translations are those
-involving lists, given lists in Isabelle are defined constructively and VDM 
-sequences map directly.      
+Even if we could avoid this translation technicality, the same problem would
+occur for recursion over non constructive types, such as sets or maps. They
+require recursion over finite sets, which are defined inductively. The only
+easy recursive translations are those involving lists, given lists in Isabelle
+are defined constructively and VDM sequences map directly.
 
-Therefore, defining recursive functions over non-constructive types entail 
-compatibility and completeness proofs.
-They also lead to partial function definitions, given Isabelle cannot 
-tell whether termination is immediately obvious. 
-In VDM, however, recursive functions on sets (as well as map domains) are common, 
-hence the need for extending our translation strategy.\<close>
+Therefore, defining recursive functions over non-constructive types entail
+compatibility and completeness proofs. They also lead to partial function
+definitions, given Isabelle cannot tell whether termination is immediately
+obvious. In VDM, however, recursive functions on sets (as well as map domains)
+are common, hence the need for extending our translation strategy.\<close>
 
 (**************************************************************************************************)
 section \<open>VDM recursion translation strategy\label{sec:Strategy}\<close>
 
-text \<open>We want to identify a translation strategy that will cater for the issues 
-described above not only for basic types, but also for sets, sequences, maps, as
-well as mutual recursion.
+text \<open>We want to identify a translation strategy that will cater for the
+issues described above not only for basic types, but also for sets, sequences,
+maps, as well as mutual recursion.
 
-The VDM AST tags all recursive functions, even those without an explicit measure. 
-All such functions will be translated using Isabelle's \<^term>\<open>fun\<close> syntax, which 
-will attempt to discover proofs for compatibility and termination. For our setup of 
-the \<^verbatim>\<open>fact\<close> example, Isabelle discovers the termination proof. 
-\<close>
+The VDM AST tags all recursive functions, even those without an explicit
+measure. All such functions will be translated using Isabelle's \<^term>\<open>fun\<close>
+syntax, which will attempt to discover proofs for compatibility and
+termination. For our setup of the \<^verbatim>\<open>fact\<close> example, Isabelle discovers the
+termination proof.\<close>
 
 (*<*)
 definition pre_fact'' :: \<open>VDMNat \<Rightarrow> \<bool>\<close> where [simp]:\<open>pre_fact'' n \<equiv> inv_VDMNat n\<close>
-fun fact'' :: \<open>VDMNat \<Rightarrow> VDMNat\<close>
-  where 
-  "fact'' n = (if pre_fact'' n then (if n = 0 then 1 else n * (fact'' (n - 1))) else undefined)" 
+fun fact'' :: \<open>VDMNat \<Rightarrow> VDMNat\<close> where 
+\<open>fact'' n = (if pre_fact'' n then (if n = 0 then 1 else n * (fact'' (n - 1))) else undefined)\<close>
 (*>*)
 
-text \<open>
-If that had failed, the user could define a VDM \<^verbatim>\<open>@IsaMeasure\<close> annotation. 
-VDM annotations are comments that will be processed according to specific implementations
-@{cite VDMJAnnotations and AdvancedVSCodePaper}. If the user does not provide an
- \<^verbatim>\<open>@IsaMeasure\<close> annotation and \<^term>\<open>fun\<close> fails, then it is up to the user to 
-figure out the necessary proof setup. 
+text \<open> If that had failed, the user could define a VDM \<^verbatim>\<open>@IsaMeasure\<close>
+annotation. VDM annotations are comments that will be processed according to
+specific implementations @{cite VDMJAnnotations and AdvancedVSCodePaper}. If
+the user does not provide an \<^verbatim>\<open>@IsaMeasure\<close> annotation and \<^term>\<open>fun\<close>
+fails, then it is up to the user to figure out the necessary proof setup.
 
-The \<^verbatim>\<open>@IsaMeasure\<close> annotation defines a well-founded measure relation that will participate in the 
-setup for Isabelle termination proof. For example, for the \<^verbatim>\<open>fact\<close> example, the 
-user would have to write an annotation before the VDM measure as
+The \<^verbatim>\<open>@IsaMeasure\<close> annotation defines a well-founded measure relation that
+will participate in the setup for Isabelle termination proof. For example, for
+the \<^verbatim>\<open>fact\<close> example, the user would have to write an annotation before the VDM
+measure as
 \begin{vdmsl}[frame=none,basicstyle=\ttfamily\scriptsize]
   --@IsaMeasure( { (n -1, n) | n : nat & n <> 0 } )
 \end{vdmsl}
-\noindent This measure relation corresponds to the relationship between the recursive 
-call (\<^verbatim>\<open>fact(n-1)\<close>) and its defining equation (\<^verbatim>\<open>fact(n)\<close>), where the 
-filtering condition determines for which values of \<^verbatim>\<open>n\<close>
-should the relation refer to. More interesting measure 
-relations are defined in Section~\ref{subsec:Complex}.  
+\noindent This measure relation corresponds to the relationship between the
+recursive call (\<^verbatim>\<open>fact(n-1)\<close>) and its defining equation (\<^verbatim>\<open>fact(n)\<close>), where
+the filtering condition determines for which values of \<^verbatim>\<open>n\<close> should the
+relation refer to. More interesting measure relations are defined in
+Section~\ref{subsec:Complex}.
 
-During translation, the plugin will typecheck the \<^verbatim>\<open>@IsaMeasure\<close> annotation 
-(\<^emph>\<open>i.e.,\<close>~it is a type correct relation over the function signature).
-Next, it will translate the annotation and some automation lemmas as a series of 
-Isabelle definitions to be used during the proof
-of termination of translated VDM recursive functions. If no annotation is provided, 
-following similar principles from Isabelle, then the plugin will try to automatically 
-infer what the measure relation should be based on the structure of the recursive 
-function definition. When this fails, then the user is informed. Still, even if
- measure-relation synthesis succeeds, the user still have to appropriately use it 
-during Isabelle's termination proof. 
+During translation, the plugin will typecheck the \<^verbatim>\<open>@IsaMeasure\<close> annotation
+(\<^emph>\<open>i.e.,\<close>~it is a type correct relation over the function signature). Next, it
+will translate the annotation and some automation lemmas as a series of
+Isabelle definitions to be used during the proof of termination of translated
+VDM recursive functions. If no annotation is provided, following similar
+principles from Isabelle, then the plugin will try to automatically infer what
+the measure relation should be based on the structure of the recursive
+function definition. When this fails, then the user is informed. Still, even
+if measure-relation synthesis succeeds, the user still have to appropriately
+use it during Isabelle's termination proof.
 
-In what follows, we will detail the translation strategy for each relevant VDM type. 
-For details over the overall translation strategy, see examples in the 
-distribution\<^footnote>\<open>\<^url>\<open>https://github.com/leouk/VDM_Toolkit\<close>\<close> and~@{cite NimFull}. That 
-is, we impose various implicit VDM checks as explicit predicates. For example, VDM 
-sets are always finite, and type invariants over set, sequence and map elements 
-must hold for every element.\<close>
+In what follows, we will detail the translation strategy for each relevant VDM
+type. For details over the overall translation strategy, see examples in the
+distribution\<^footnote>\<open>\<^url>\<open>https://github.com/leouk/VDM_Toolkit\<close>\<close> and~@{cite NimFull}.
+That is, we impose various implicit VDM checks as explicit predicates. For
+example, VDM sets are always finite, and type invariants over set, sequence
+and map elements must hold for every element.\<close>
 
 (*-------------------------------------------------------------------------------------------------*)
 subsection \<open>Recursion over VDM basic types (\<^bold>\<open>nat\<close>, \<^bold>\<open>int\<close>)\label{subsec:VDMNat}\<close>
 
-text \<open>Following the general translation strategy~@{cite NimFull}, 
-we first encode the implicit precondition as a simplification rule, 
-which insists that the given parameter \<^term>\<open>n\<close> is a \<^typ>\<open>VDMNat\<close>, alongside a 
-list of defining constants that are useful for proof strategy synthesis.\<close>
+text \<open>Following the general translation strategy~@{cite NimFull}, we first
+encode the implicit precondition as a simplification rule, which insists that
+the given parameter \<^term>\<open>n\<close> is a \<^typ>\<open>VDMNat\<close>, alongside a list of
+defining constants that are useful for proof strategy synthesis.\<close>
 
 definition pre_fact :: \<open>VDMNat \<Rightarrow> \<bool>\<close> where [simp]:\<open>pre_fact n \<equiv> inv_VDMNat n\<close>
 lemmas pre_fact_defs = pre_fact_def inv_VDMNat_def 
 
-text \<open>Next, we define factorial recursively. When the precondition fails, 
-  we return \<^term>\<open>undefined\<close>, which is a term that cannot be reasoned with in Isabelle 
-The \<^term>\<open>domintros\<close> tag tells Isabelle to generate domain predicates, in case this function is not total. 
-Domain predicates are important to our strategy because every VDM function will be undefined, when
-applied outside its precondition. It also generates domain-predicate sensitive proof rules listed below.\<close>
+text \<open>Next, we define factorial recursively. When the precondition fails, we
+return \<^term>\<open>undefined\<close>, which is a term that cannot be reasoned with in
+Isabelle The \<^term>\<open>domintros\<close> tag tells Isabelle to generate domain
+predicates, in case this function is not total. Domain predicates are
+important to our strategy because every VDM function will be undefined, when
+applied outside its precondition. It also generates domain-predicate sensitive
+proof rules listed below.\<close>
 function (domintros) fact :: \<open>VDMNat \<Rightarrow> VDMNat\<close> where
 \<open>fact n = (if pre_fact n then (if n = 0 then 1 else n * (fact (n - 1))) else undefined)\<close>
 
-  text \<open>The proof obligations for pattern compatibility and completeness are 
-discharged with the usual Isabelle proof strategy for simple recursive patterns with the @{method pat_completeness} method.
-  In the general case discussed in Section~\ref{subsec:Complex}), 
-  the user might have goals to discharge.\<close>
+text \<open>The proof obligations for pattern compatibility and completeness are
+discharged with the usual Isabelle proof strategy for simple recursive
+patterns with the @{method pat_completeness} method. In the general case
+discussed in Section~\ref{subsec:Complex}), the user might have goals to
+discharge.\<close>
   by (pat_completeness, auto) \<^marker>\<open>tag invisible\<close>
-
-text \<open>Various theorems are made available, such as: case analysis; and (partial) rules
-for elimination, induction and simplification.
-%Case analysis @{thm fact.cases}
-%Elimination rules (partial) @{thm fact.pelims}
-%Induction rules (partial) @{thm fact.pinduct}
-%Simplification rules (partial) @{thm fact.psimps}
+  
+text \<open>Various theorems are made available, such as: case analysis; and
+(partial) rules for elimination, induction and simplification. %Case analysis
+@{thm fact.cases} %Elimination rules (partial) @{thm fact.pelims} %Induction
+rules (partial) @{thm fact.pinduct} %Simplification rules (partial) @{thm
+fact.psimps}
 
 Note the last two are partial, module the domain predicate @{term fact_dom},
-which represents a well-founded relation that ensures termination. That is, if the user does not want
-(or knows how) to prove termination, such domain predicates will follow every application of the 
-\<^term>\<open>fact\<close> definition, hence imposing users the requirement that such well-founded relation is still missing.
+which represents a well-founded relation that ensures termination. That is, if
+the user does not want (or knows how) to prove termination, such domain
+predicates will follow every application of the \<^term>\<open>fact\<close> definition,
+hence imposing users the requirement that such well-founded relation is still
+missing.
 
-If/when the termination proof is discharged, these p-rules can be simplified into total rules that 
-do not depend on a domain predicate, given a well-founded relation has been provided. Domain predicates
-will complicate user proofs, and also make proof strategy synthesis harder to automate.
+If/when the termination proof is discharged, these p-rules can be simplified
+into total rules that do not depend on a domain predicate, given a
+well-founded relation has been provided. Domain predicates will complicate
+user proofs, and also make proof strategy synthesis harder to automate.
 
-Termination proof is discharged by establishing a well-founded relation associated with 
-the function recursive call(s) with respect to its declaration. In our case, the \<^verbatim>\<open>@IsaMeasure\<close>
-annotation is translated as an Isabelle abbreviation. We also implicitly add the filter that the 
-function precondition holds:~this is important to ensure the termination proof never reaches the \<^term>\<open>undefined\<close> case.  
-The other filter comes from the negated test in the definition if-statement. More complex definitions will
-have more involved filters. 
-We use abbreviation instead of definition to avoid needing to expand the defined term.\<close>
+Termination proof is discharged by establishing a well-founded relation
+associated with the function recursive call(s) with respect to its
+declaration. In our case, the \<^verbatim>\<open>@IsaMeasure\<close> annotation is translated as an
+Isabelle abbreviation. We also implicitly add the filter that the function
+precondition holds:~this is important to ensure the termination proof never
+reaches the \<^term>\<open>undefined\<close> case. The other filter comes from the negated
+test in the definition if-statement. More complex definitions will have more
+involved filters. We use abbreviation instead of definition to avoid needing
+to expand the defined term.\<close>
 
 abbreviation fact_wf :: \<open>(VDMNat \<times> VDMNat) set\<close> where
   \<open>fact_wf \<equiv> { (n - 1, n) | n . pre_fact n \<and> n \<noteq> 0 }\<close>
 
-text \<open>Given \<^term>\<open>fact\<close> is a simple (non-mutual, single call-site, easy measure relation choice) recursion, 
-  thankfully the setup is not as complex to establish well-foundedness. For recursions of this nature, we can 
-  piggyback on some Isabelle machinery to help prove well foundedness by using the terms @{term gen_VDMNat_term} and
-  @{term int_ge_less_than}.
+text \<open>Given \<^term>\<open>fact\<close> is a simple (non-mutual, single call-site, easy
+measure relation choice) recursion, thankfully the setup is not as complex to
+establish well-foundedness. For recursions of this nature, we can piggyback on
+some Isabelle machinery to help prove well foundedness by using the terms
+@{term gen_VDMNat_term} and @{term int_ge_less_than}.
 
-  The first term is defined in terms of the second, which is a subset of our well-formed relation \<^term>\<open>fact_wf\<close>. 
-  Isabelle has proofs about the term's well formedness of \<^term>\<open>int_ge_less_than\<close>.
-  Thus, making the proof our term being well-founded trivial, and easily discovered with proof tools like
-  @{command sledgehammer}. As part of the translation strategy, we then define (and automatically discover the proof of)
-  the following lemma. This follows the strategy described in~@{cite KrausSCNP}. 
-    %\url{https://www21.in.tum.de/~krauss/papers/scnp-wst.pdf}.\<close>
+The first term is defined in terms of the second, which is a subset of our
+well-formed relation \<^term>\<open>fact_wf\<close>. Isabelle has proofs about the term's
+well formedness of \<^term>\<open>int_ge_less_than\<close>. Thus, making the proof our
+term being well-founded trivial, and easily discovered with proof tools like
+@{command sledgehammer}. As part of the translation strategy, we then define
+(and automatically discover the proof of) the following lemma. This follows
+the strategy described in~@{cite KrausSCNP}.    
+%\url{https://www21.in.tum.de/~krauss/papers/scnp-wst.pdf}.\<close>
 lemma l_fact_term_wf: \<open>wf (gen_VDMNat_term fact_wf)\<close>
   by (simp add: wf_int_ge_less_than wf_Int1) 
 
+text \<open>Finally, we prove termination using the previously proved lemma using
+the @{method relation}. This simplifies the goal into well-formedness of
+termination relation and that the precondition implies it, both of which are
+easily proved with simplification in this case.\<close>
 termination \<^marker>\<open>tag invisible\<close>
-  text \<open>Finally, we prove termination using the previously proved lemma using the @{method relation}.
-  This simplifies the goal into well-formedness of termination relation and that the precondition implies it,
-  both of which are easily proved with simplification in this case.\<close>
   apply (relation \<open>(gen_VDMNat_term fact_wf)\<close>) \<^marker>\<open>tag invisible\<close>
-  text \<open>This transforms the abstract domain predicate into two new subgoals as @{subgoals[display]}\<close>
+text \<open>This transforms the abstract domain predicate into two new subgoals as
+@{subgoals[display]}\<close>
   using l_fact_term_wf apply presburger \<^marker>\<open>tag invisible\<close>
   by (simp add: int_ge_less_than_def) \<^marker>\<open>tag invisible\<close>
 
-text \<open>For this simple example, these subgoals are proved with @{command sledgehammer}. In general, the user will be
-  have to either find the proof, or deal with domain predicates in proofs involving the recursive call.
- After the termination proof is discharged, Isabelle provides versions of rules 
-for elimination, induction and simplification that are total and do not depend on 
+text \<open>For this simple example, these subgoals are proved with @{command
+sledgehammer}. In general, the user will be have to either find the proof, or
+deal with domain predicates in proofs involving the recursive call. After the
+termination proof is discharged, Isabelle provides versions of rules for
+elimination, induction and simplification that are total and do not depend on
 the abstract domain predicate. 
-\<close>
 
-text \<open>To make sure our choice does not lead to the empty relation, we ensure
-  that indeed the termination relation is in fact the same as the well founded predicate by proving the next goal.
-  This is something users might want to do, but is not part of the translation strategy. In case the measure relation 
-  is empty, the recursive call simplification rules will not be useful anyhow.\<close>
+To make sure our choice does not lead to the empty relation, we ensure that
+indeed the termination relation is in fact the same as the well founded
+predicate by proving the next goal. This is something users might want to do,
+but is not part of the translation strategy. In case the measure relation is
+empty, the recursive call simplification rules will not be useful anyhow.\<close>
+
 lemma l_fact_term_valid: \<open>(gen_VDMNat_term fact_wf) = fact_wf\<close>
   apply (simp ) \<^marker>\<open>tag invisible\<close>
   apply (intro equalityI subsetI)\<^marker>\<open>tag invisible\<close>
@@ -337,8 +370,9 @@ lemma l_fact_term_valid: \<open>(gen_VDMNat_term fact_wf) = fact_wf\<close>
 (*-------------------------------------------------------------------------------------------------*)
 subsection \<open>Recursion over VDM sets\label{subsec:VDMSet}\<close>
 
-text \<open>Next, we extend the translation strategy for basic types for VDM sets. For this, we will use a 
- recursively defined VDM function over sets that sums the set elements as
+text \<open>Next, we extend the translation strategy for basic types for VDM sets.
+For this, we will use a recursively defined VDM function over sets that sums
+the set elements as
 %
 \begin{vdmsl}[frame=none,basicstyle=\ttfamily\scriptsize]
   sumset: set of nat -> nat 
@@ -348,80 +382,92 @@ text \<open>Next, we extend the translation strategy for basic types for VDM set
   measure card s;
 \end{vdmsl}
 %
-\noindent Like most common VDM recursion over sets, the function consumes the set by picking each 
-set element and them calling the recursive call without the element picked, until the set is empty. 
-The VDM measure states that the recursion is based on the cardinality of the input parameter. VDM 
-measures are not suitable for Isabelle proofs, given Isabelle requires a relation;~hence,
-VDM measures are ignored during translation. They might still be useful during proofs as potential 
-witnesses to existentially-quantified goals.
+\noindent Like most common VDM recursion over sets, the function consumes the
+set by picking each set element and them calling the recursive call without
+the element picked, until the set is empty. The VDM measure states that the
+recursion is based on the cardinality of the input parameter. VDM measures are
+not suitable for Isabelle proofs, given Isabelle requires a relation;~hence,
+VDM measures are ignored during translation. They might still be useful during
+proofs as potential witnesses to existentially-quantified goals.
 
-In Isabelle, the implicit VDM checks are defined as the precondition, which ensures 
-that the given set contains only natural numbers, and is finite, as defined by \<^term>\<open>inv_VDMSet'\<close>\<close>
+In Isabelle, the implicit VDM checks are defined as the precondition, which
+ensures that the given set contains only natural numbers, and is finite, as
+defined by \<^term>\<open>inv_VDMSet'\<close>\<close>
 
 definition pre_sumset :: \<open>VDMNat VDMSet \<Rightarrow> \<bool>\<close> where
   \<open>pre_sumset s \<equiv> inv_VDMSet' inv_VDMNat s\<close>
 lemmas pre_sumset_defs = pre_sumset_def inv_VDMSet'_defs inv_VDMNat_def
 
-text \<open>We define the VDM recursive function in Isabelle next. It checks whether the given
-      set satisfy the function precondition, returning \<^term>\<open>undefined\<close> if not.
-      Each case is encoded pretty much 1-1 from VDM after that. The translation strategy for
-      VDM \<^verbatim>\<open>let-in-set\<close> patterns uses Isabelle's Hilbert's choice operator (\<^term>\<open>\<some> x . x \<in> s\<close>).
-    Note this naturally extends to VDM's \<^verbatim>\<open>let-be-st\<close> patterns as well.\<close>
+text \<open>We define the VDM recursive function in Isabelle next. It checks whether
+the given set satisfy the function precondition, returning \<^term>\<open>undefined\<close>
+if not. Each case is encoded pretty much 1-1 from VDM after that. The
+translation strategy for VDM \<^verbatim>\<open>let-in-set\<close> patterns uses Isabelle's Hilbert's
+choice operator (\<^term>\<open>\<some> x . x \<in> s\<close>). Note this naturally extends to VDM's
+\<^verbatim>\<open>let-be-st\<close> patterns as well.\<close>
 function (domintros) sumset :: \<open>VDMNat VDMSet \<Rightarrow> VDMNat\<close> where 
   \<open>sumset s = (if pre_sumset s then 
                    (if s = {} then 0 else let e = (\<some> x . x \<in> s) in sumset (s - {e}) + e) 
                   else undefined)\<close>
-  text \<open>The pattern completeness and compatibility goals are discharged with 
-  the usual proof strategy of @{method pat_completeness}.
-        For more general examples, if that fails, @{command sledgehammer} should be used.\<close>
+text \<open>The pattern completeness and compatibility goals are discharged with
+the usual proof strategy of @{method pat_completeness}. For more general
+examples, if that fails, @{command sledgehammer} should be used.\<close>
   by (pat_completeness, auto) \<^marker>\<open>tag invisible\<close>
 
-text \<open>The measure relation for termination is defined with the \<^verbatim>\<open>@IsaMeasure\<close> annotation above as 
-   the smaller set after picking \<^term>\<open>e\<close> (\<^emph>\<open>e.g.,\<close>~\<^term>\<open>s - {(\<some> e . e \<in> s)}\<close>), 
-    and the set used at the entry call, leading to the pairs \<^term>\<open>(s - {(\<some> e . e \<in> s)}, s)\<close>. 
-    Finally, we ensure all the relation elements satisfy the function precondition (\<^term>\<open>pre_sumset\<close>),
-   and that the if-test is negated.
-\<close>
+text \<open>The measure relation for termination is defined with the \<^verbatim>\<open>@IsaMeasure\<close>
+annotation above as the smaller set after picking \<^term>\<open>e\<close>
+(\<^emph>\<open>e.g.,\<close>~\<^term>\<open>s - {(\<some> e . e \<in> s)}\<close>), and the set used at the entry call,
+leading to the pairs \<^term>\<open>(s - {(\<some> e . e \<in> s)}, s)\<close>. Finally, we ensure
+all the relation elements satisfy the function precondition
+(\<^term>\<open>pre_sumset\<close>), and that the if-test is negated. \<close>
 abbreviation sumset_wf_rel :: \<open>(VDMNat VDMSet \<times> VDMNat VDMSet) set\<close> where
   \<open>sumset_wf_rel \<equiv> { (s - {(\<some> e . e \<in> s)}, s)| s . pre_sumset s \<and> s \<noteq> {}}\<close>
 
-text \<open>Given this is a simple (non-mutual, single call-site, easy set element choice) recursion, again
-   we can piggyback on Isabelle machinery by using the terms @{term gen_set_term} and 
-   @{term finite_psubset}
+text \<open>Given this is a simple (non-mutual, single call-site, easy set element
+choice) recursion, again we can piggyback on Isabelle machinery by using the
+terms @{term gen_set_term} and @{term finite_psubset}.
 
-  They establishes that a relation where the first element is strictly smaller set than the 
-  second element in the relation pair is well-formed. This makes the proof of well-foundedness easy 
-  for \<^term>\<open>sumset_wf_rel\<close> through @{command sledgehammer}. \<close>
+They establishes that a relation where the first element is strictly smaller
+set than the second element in the relation pair is well-formed. This makes
+the proof of well-foundedness easy for \<^term>\<open>sumset_wf_rel\<close> through
+@{command sledgehammer}. \<close>
+
 lemma l_sumset_rel_wf: \<open>wf (gen_set_term sumset_wf_rel)\<close>
   using l_gen_set_term_wf \<^marker>\<open>tag invisible\<close>
   by blast \<^marker>\<open>tag invisible\<close>
 
+text \<open>Next, we tackle the termination proof, with the same setup with @{method
+relation} again.\<close>
 termination\<^marker>\<open>tag invisible\<close>
-  text \<open>Next, we tackle the termination proof, with the same setup with @{method relation} again.\<close>
   apply (relation \<open>(gen_set_term sumset_wf_rel)\<close>)\<^marker>\<open>tag invisible\<close>
   using l_sumset_rel_wf \<^marker>\<open>tag invisible\<close> 
   apply force\<^marker>\<open>tag invisible\<close>
-  text \<open>Unfortunately, using @{command sledgehammer} fails to discharge the second subgoal @{subgoals[display]}\<close>
+  text \<open>Unfortunately, using @{command sledgehammer} fails to discharge the
+  second subgoal @{subgoals[display]}\<close>
   oops\<^marker>\<open>tag invisible\<close>
 
-  text \<open>Fortunately, for most simple situations, this is easy to decompose in general. The translation strategy takes the 
-    \<^verbatim>\<open>@IsaMeasure\<close> expression and decompose its parts, such that the filtering predicates are assumptions, and
-    the element in the relation belong to the well-formed measure chosen. For the concrete set example, this is defined 
-  in the next lemma, which require some manual intervention to tell Isabelle what definitions to unfold and simplify with. 
-  Then, Isabelle's @{command sledgehammer} can finish the proof.\<close>
-
+text \<open>Fortunately, for most simple situations, this is easy to decompose in
+general. The translation strategy takes the \<^verbatim>\<open>@IsaMeasure\<close> expression and
+decompose its parts, such that the filtering predicates are assumptions, and
+the element in the relation belong to the well-formed measure chosen. For
+the concrete set example, this is defined in the next lemma, which require
+some manual intervention to tell Isabelle what definitions to unfold and
+simplify with. Then, Isabelle's @{command sledgehammer} can finish the
+proof.\<close>
 lemma l_pre_sumset_sumset_wf_rel: 
   \<open>pre_sumset s \<Longrightarrow> s \<noteq> {} \<Longrightarrow> (s - {(\<some> x. x \<in> s)}, s) \<in> (gen_set_term sumset_wf_rel)\<close>
   unfolding gen_set_term_def \<^marker>\<open>tag invisible\<close>
   apply (simp add: pre_sumset_defs)\<^marker>\<open>tag invisible\<close>
   by (metis Diff_subset member_remove psubsetI remove_def some_in_eq)\<^marker>\<open>tag invisible\<close>
 
-text \<open>The intuition behind this lemma is that, elements in the measure relation satisfy well-formedness under the function 
-  precondition and the filtering case (\<^term>\<open>s \<noteq> {}\<close>) where the recursive call is made. That is, the precondition and 
-  filtering condition help establish the terminating relation. For this particular proof, the only aspect needed from the 
-  precondition (\<^term>\<open>pre_sumset\<close>) is that the set is finite. 
+text \<open>The intuition behind this lemma is that, elements in the measure
+relation satisfy well-formedness under the function precondition and the
+filtering case (\<^term>\<open>s \<noteq> {}\<close>) where the recursive call is made. That is,
+the precondition and filtering condition help establish the terminating
+relation. For this particular proof, the only aspect needed from the
+precondition (\<^term>\<open>pre_sumset\<close>) is that the set is finite.
 
-  With this, we can try the termination proof again, which now @{command sledgehammer} find proofs for all subgoals.\<close>
+With this, we can try the termination proof again, which now @{command
+sledgehammer} find proofs for all subgoals.\<close>
 termination\<^marker>\<open>tag invisible\<close>
   apply (relation \<open>(gen_set_term sumset_wf_rel)\<close>)\<^marker>\<open>tag invisible\<close>
   using l_sumset_rel_wf apply force\<^marker>\<open>tag invisible\<close>
@@ -431,29 +477,38 @@ lemma l_pre_fact_wf_rel': "pre_fact n \<Longrightarrow> n \<noteq> 0 \<Longright
   unfolding gen_VDMNat_term_def gen_VDMInt_term_def
   using l_fact_term_valid by force
 (*>*)
-text \<open>Note we omit such lemma over termination and precondition for the \<^typ>\<open>VDMNat\<close> case in Section~\ref{subsec:VDMNat}. 
-  The translation strategy does define it following the same recipe:~recursive function precondition and filtering predicate 
-  as assumptions, and chosen termination relation element containment, where @{command sledgehammer} find the proof once more.\<close>
+
+text \<open>Note we omit such lemma over termination and precondition for the
+\<^typ>\<open>VDMNat\<close> case in Section~\ref{subsec:VDMNat}. The translation strategy
+does define it following the same recipe:~recursive function precondition and
+filtering predicate as assumptions, and chosen termination relation element
+containment, where @{command sledgehammer} find the proof once more.\<close>
 lemma l_pre_fact_wf_rel: \<open>\<lbrakk>pre_fact n; n \<noteq> 0\<rbrakk> \<Longrightarrow> (n - 1, n) \<in> gen_VDMNat_term fact_wf\<close>
   unfolding gen_VDMNat_term_def gen_VDMInt_term_def \<^marker>\<open>tag invisible\<close>
-  using inv_VDMNat_def l_less_than_VDMNat_subset_int_ge_less_than pre_fact_def by auto \<^marker>\<open>tag invisible\<close>
+  using inv_VDMNat_def l_less_than_VDMNat_subset_int_ge_less_than pre_fact_def \<^marker>\<open>tag invisible\<close>
+  by auto \<^marker>\<open>tag invisible\<close>
 
-text \<open>We also choose to show the relation finite subset trick to
-make well-founded induction proofs easier does not compromise the well founded relation itself.\<close>
+text \<open>We also choose to show the relation finite subset trick to make
+well-founded induction proofs easier does not compromise the well founded
+relation itself.\<close>
 lemma l_sumset_wf_rel_valid: \<open>gen_set_term sumset_wf_rel = sumset_wf_rel\<close>
   apply (intro equalityI subsetI, simp) \<^marker>\<open>tag invisible\<close>
   using l_pre_sumset_sumset_wf_rel by blast \<^marker>\<open>tag invisible\<close>
 
-text \<open>Finally, even though this was not necessary for this proof, we encourage users to always provide a witness for the top recursive call.
-  This is done by using the \<^verbatim>\<open>@Witness\<close> annotation~@{cite EdwardWitness and AdvancedVSCodePaper}:~it provides a concrete example for the function 
-  input parameters. This witness is useful for existentially quantified predicates present in more involved termination proofs (see Section~\ref{subsec:Complex}).\<close>
+text \<open>Finally, even though this was not necessary for this proof, we encourage
+users to always provide a witness for the top recursive call. This is done by
+using the \<^verbatim>\<open>@Witness\<close> annotation~@{cite EdwardWitness and
+AdvancedVSCodePaper}:~it provides a concrete example for the function input
+parameters. This witness is useful for existentially quantified predicates
+present in more involved termination proofs (see
+Section~\ref{subsec:Complex}).\<close>
 
 (*-------------------------------------------------------------------------------------------------*)
 subsection \<open>Recursion over VDM maps\label{subsec:VDMMap}\<close>
 
-text \<open>Recursive functions over VDM maps are a special case of VDM sets, given map recursion usually 
-iterates over the map's domain. For example, the function that sums the elements of the map range 
-can be defined as  
+text \<open>Recursive functions over VDM maps are a special case of VDM sets, given
+map recursion usually iterates over the map's domain. For example, the
+function that sums the elements of the map range can be defined as
 %
 \begin{vdmsl}[frame=none,basicstyle=\ttfamily\scriptsize]
   sum_elems: map nat to nat -> nat
@@ -465,25 +520,32 @@ can be defined as
   measure card dom m;
 \end{vdmsl}
 %
-\noindent As with sets, it iterates over the map by picking a domain element, performing the necessary 
-computation, and then recurse on the map filtered by removing the chosen element, until the map is 
-empty and the function terminates. As before, the measure relation follows the same pattern:~recursive call 
-site related with defining site, where both the if-test and the \<^verbatim>\<open>let-in-set\<close> choice is part of the filtering predicate.
+\noindent As with sets, it iterates over the map by picking a domain element,
+performing the necessary computation, and then recurse on the map filtered by
+removing the chosen element, until the map is empty and the function
+terminates. As before, the measure relation follows the same
+pattern:~recursive call site related with defining site, where both the
+if-test and the \<^verbatim>\<open>let-in-set\<close> choice is part of the filtering predicate.
 
-Following the general translation strategy for maps~@{cite NimFull}, we define the function precondition using \<^term>\<open>inv_Map\<close>
-It insists that both the map domain and range are finite, and that all domain and range elements satisfy their corresponding type invariant. 
-Note that if the recursion was defined over sets other than the domain and range, Isabelle might require you to prove such set is finite. 
-Given both domain and range sets are themselves finite, this should be easy enough to do, if needed. 
-\<close>
+Following the general translation strategy for maps~@{cite NimFull}, we define
+the function precondition using \<^term>\<open>inv_Map\<close> It insists that both the map
+domain and range are finite, and that all domain and range elements satisfy
+their corresponding type invariant. Note that if the recursion was defined
+over sets other than the domain and range, Isabelle might require you to prove
+such set is finite. Given both domain and range sets are themselves finite,
+this should be easy enough to do, if needed.\<close>
+
 definition pre_sum_elems :: \<open>(VDMNat \<rightharpoonup> VDMNat) \<Rightarrow> \<bool>\<close> where
   \<open>pre_sum_elems m \<equiv> inv_Map inv_VDMNat inv_VDMNat m\<close>
 lemmas pre_sum_elems_defs = pre_sum_elems_def inv_Map_defs inv_VDMNat_def 
 
-text \<open>VDM maps in Isabelle (\<^typ>\<open>(VDMNat \<rightharpoonup> VDMNat)\<close>) are defined as a HOL function which maps to an optional result. 
-That is, if the element is in the domain, the map results in a non {\texttt{\<^bold>\<open>nil\<close>}} value, whereas if the element
-does not belong to the domain, the map results in a {\texttt{\<^bold>\<open>nil\<close>}} value. This effectively makes all maps total,
-where values outside the domain map to {\texttt{\<^bold>\<open>nil\<close>}}. The Isabelle translation and compatibility proof follows 
-patterns used before and are given as\<close>
+text \<open>VDM maps in Isabelle (\<^typ>\<open>(VDMNat \<rightharpoonup> VDMNat)\<close>) are defined as a HOL
+function which maps to an optional result. That is, if the element is in the
+domain, the map results in a non {\texttt{\<^bold>\<open>nil\<close>}} value, whereas if the
+element does not belong to the domain, the map results in a {\texttt{\<^bold>\<open>nil\<close>}}
+value. This effectively makes all maps total, where values outside the domain
+map to {\texttt{\<^bold>\<open>nil\<close>}}. The Isabelle translation and compatibility proof
+follows patterns used before and are given as\<close>
 function (domintros) sum_elems :: \<open>(VDMNat \<rightharpoonup> VDMNat) \<Rightarrow> VDMNat\<close> where
   \<open>sum_elems m = (if pre_sum_elems m then
                       if m = Map.empty then 0 else
@@ -491,22 +553,27 @@ function (domintros) sum_elems :: \<open>(VDMNat \<rightharpoonup> VDMNat) \<Rig
                   else undefined)\<close>
   by (pat_completeness, auto) \<^marker>\<open>tag invisible\<close>
 
-text \<open>Similarly, the well-formed relation from \<^verbatim>\<open>@IsaMeasure\<close> is translated next, where the precondition is also included 
-as part of the relation's filter. The \<^term>\<open>{d}-\<triangleleft>m\<close> corresponds to VDM domain anti-filtering operator \<^verbatim>\<open><-:\<close>.\<close>
+text \<open>Similarly, the well-formed relation from \<^verbatim>\<open>@IsaMeasure\<close> is translated
+next, where the precondition is also included as part of the relation's
+filter. The \<^term>\<open>{d}-\<triangleleft>m\<close> corresponds to VDM domain anti-filtering operator
+\<^verbatim>\<open>{d}<-:m\<close>.\<close>
 abbreviation sum_elems_wf :: \<open>((VDMNat \<rightharpoonup> VDMNat) \<times> (VDMNat \<rightharpoonup> VDMNat)) VDMSet\<close> where
   \<open>sum_elems_wf \<equiv> 
   { (({d} -\<triangleleft> m), m) | m d . pre_sum_elems m \<and> m \<noteq> Map.empty \<and> d \<in> dom m }\<close>
 
-text \<open>For the well-formed lemma over the recursive measure relation, there are no available Isabelle help, 
-and projecting the domain element of the maps within the relation is awkward. Thus, we have to prove the 
-lemma directly. This will not be automatic in general. This is one difference in terms of translation of VDM 
-recursive functions over sets and maps.
+text \<open>For the well-formed lemma over the recursive measure relation, there are
+no available Isabelle help, and projecting the domain element of the maps
+within the relation is awkward. Thus, we have to prove the lemma directly.
+This will not be automatic in general. This is one difference in terms of
+translation of VDM recursive functions over sets and maps.
 
-Fortunately, the proof strategy for such situations is somewhat known:~it follows a similar strategy to
-the proof of well formedness of the \<^term>\<open>finite_psubset\<close> as @{thm wf_finite_psubset}. The proof uses
-the VDM measure expression to extract the right projection of interest, then follows the proof for \<^term>\<open>finite_psubset\<close>. 
-Finally, @{command sledgehammer} can figure out the final steps.   
-\<close>
+Fortunately, the proof strategy for such situations is somewhat known:~it
+follows a similar strategy to the proof of well formedness of the
+\<^term>\<open>finite_psubset\<close> as @{thm wf_finite_psubset}. The proof uses the VDM
+measure expression to extract the right projection of interest, then follows
+the proof for \<^term>\<open>finite_psubset\<close>. Finally, @{command sledgehammer} can
+figure out the final steps.\<close>
+
 lemma l_sum_elems_wf: \<open>wf sum_elems_wf\<close>
   apply (rule wf_measure[of \<open>\<lambda> m . card (dom m)\<close>, THEN wf_subset]) \<^marker>\<open>tag invisible\<close>
   apply (simp add: measure_def inv_image_def less_than_def less_eq)\<^marker>\<open>tag invisible\<close>
@@ -514,8 +581,9 @@ lemma l_sum_elems_wf: \<open>wf sum_elems_wf\<close>
   apply (elim exE conjE)\<^marker>\<open>tag invisible\<close>
   by (simp add: l_VDMMap_filtering_card pre_sum_elems_defs)\<^marker>\<open>tag invisible\<close>
 
-text \<open>The precondition subgoal and the termination proof follow the same patterns as before. Again,
-their proof was discovered with @{command sledgehammer}, yet this will not be the case in general.\<close>
+text \<open>The precondition subgoal and the termination proof follow the same
+patterns as before. Again, their proof was discovered with @{command
+sledgehammer}, yet this will not be the case in general.\<close>
 lemma l_pre_sum_elems_sum_elems_wf: \<open>\<lbrakk>pre_sum_elems m; m \<noteq> Map.empty\<rbrakk> \<Longrightarrow> ({(\<some> e. e \<in> dom m)} -\<triangleleft> m, m) \<in> sum_elems_wf\<close>
   apply (simp add: pre_sum_elems_defs) \<^marker>\<open>tag invisible\<close>
   by (metis domIff empty_iff some_in_eq) \<^marker>\<open>tag invisible\<close>
@@ -526,9 +594,11 @@ termination  \<^marker>\<open>tag invisible\<close>
   apply (simp add: l_sum_elems_wf)\<^marker>\<open>tag invisible\<close>
   using l_pre_sum_elems_sum_elems_wf by presburger\<^marker>\<open>tag invisible\<close>
 
-text \<open>Finally, we also prove that the well founded termination relation (\<^term>\<open>sum_elems_wf\<close>) is not 
-empty, as we did for sets and \<^bold>\<open>nat\<close> recursion. Note that here the \<^verbatim>\<open>@Witness\<close> annotation is 
-useful in discharging the actual value to use as the witness demonstrating the relation is not empty.\<close>
+text \<open>Finally, we also prove that the well founded termination relation
+(\<^term>\<open>sum_elems_wf\<close>) is not empty, as we did for sets and \<^bold>\<open>nat\<close>
+recursion. Note that here the \<^verbatim>\<open>@Witness\<close> annotation is useful in discharging
+the actual value to use as the witness demonstrating the relation is not
+empty.\<close>
 lemma l_sum_elems_wf_valid: \<open>sum_elems_wf \<noteq> {}\<close>
   apply safe \<^marker>\<open>tag invisible\<close>
   apply (erule equalityE)\<^marker>\<open>tag invisible\<close>
@@ -539,17 +609,17 @@ lemma l_sum_elems_wf_valid: \<open>sum_elems_wf \<noteq> {}\<close>
 (*-------------------------------------------------------------------------------------------------*)
 subsection \<open>VDM recursion involving complex measures\label{subsec:Complex}\<close>
 
-text \<open>The class of recursive examples shown so far have cover a wide range of 
-situations, and have a good level of automation. Nevertheless, the same strategy can
-also be applied for me complex recursive definitions. The cost for the VDM user
-is the need of a more involved \<^verbatim>\<open>@IsaMeasure\<close> definition and the highly likely need for
-extra user-defined lemmas. These lemmas can be defined in VDM itself using 
-the \<^verbatim>\<open>@Lemma\<close> annotation, which will be translated to Isabelle as any other boolean 
-expression would.
+text \<open>The class of recursive examples shown so far have cover a wide range of
+situations, and have a good level of automation. Nevertheless, the same
+strategy can also be applied for me complex recursive definitions. The cost
+for the VDM user is the need of a more involved \<^verbatim>\<open>@IsaMeasure\<close> definition and
+the highly likely need for extra user-defined lemmas. These lemmas can be
+defined in VDM itself using the \<^verbatim>\<open>@Lemma\<close> annotation, which will be translated
+to Isabelle as any other boolean expression would.
 
-To illustrate this, we define in VDM the (in)famous Ackermann 
-function\<^footnote>\<open>\<^url>\<open>https://en.wikipedia.org/wiki/Ackermann_function\<close>\<close>, 
-which is a staple example of complex recursion, as  
+To illustrate this, we define in VDM the (in)famous Ackermann
+function\<^footnote>\<open>\<^url>\<open>https://en.wikipedia.org/wiki/Ackermann_function\<close>\<close>, which is a
+staple example of complex recursion, as
 %
 \begin{vdmsl}[frame=none,basicstyle=\ttfamily\scriptsize]
     ack: nat * nat -> nat 
@@ -561,21 +631,23 @@ which is a staple example of complex recursion, as
     measure is not yet specified;
 \end{vdmsl}
 %
-\noindent Note that the VDM measure is not defined, and that the \<^verbatim>\<open>@IsaMeasure\<close>
-uses a construct from Isabelle called \<^term>\<open>pair_less\<close>. It is part of Isabelle's 
-machinery of concrete orders for SCNP problems @{cite KrausSCNP}. 
-It considers recursions over multiple parameters, where some might 
-increase the number of calls (\<^emph>\<open>e.g.\<close>~size-change). We are not aware of a 
-mechanism to define such measures in VDM. 
+\noindent Note that the VDM measure is not defined, and that the
+\<^verbatim>\<open>@IsaMeasure\<close> uses a construct from Isabelle called \<^term>\<open>pair_less\<close>. It
+is part of Isabelle's machinery of concrete orders for SCNP problems @{cite
+KrausSCNP}. It considers recursions over multiple parameters, where some might
+increase the number of calls (\<^emph>\<open>e.g.\<close>~size-change). We are not aware of a
+mechanism to define such measures in VDM.
 
-We instantiate \<^term>\<open>pair_less\<close> to \<^typ>\<open>VDMNat\<close>. It is defined as the lexicographic 
-product over the transitive closure of a totally ordered relation between \<^typ>\<open>VDMNat\<close> 
-inputs\<^footnote>\<open>Details of this definition in the \<^verbatim>\<open>VDMToolkit.thy\<close> file within the 
-distribution in~\<^url>\<open>https://github.com/leouk/VDM_Toolkit\<close>.\<close>. 
+We instantiate \<^term>\<open>pair_less\<close> to \<^typ>\<open>VDMNat\<close>. It is defined as the
+lexicographic product over the transitive closure of a totally ordered
+relation between \<^typ>\<open>VDMNat\<close> inputs\<^footnote>\<open>Details of this definition in the
+\<^verbatim>\<open>VDMToolkit.thy\<close> file within the distribution
+in~\<^url>\<open>https://github.com/leouk/VDM_Toolkit\<close>.\<close>.
 
-If VDM measures were over relations, the Ackermann measure could be defined defined in VDM,
-assuming a standard definition of transitive closure\<^footnote>\<open>The \<^verbatim>\<open>Relations.vdmsl\<close> provides 
-such definition in the VDM toolkit distribution.\<close>, as
+If VDM measures were over relations, the Ackermann measure could be defined
+defined in VDM, assuming a standard definition of transitive closure\<^footnote>\<open>The
+\<^verbatim>\<open>Relations.vdmsl\<close> provides such definition in the VDM toolkit distribution.\<close>,
+as
 %
 \begin{vdmsl}[frame=none,basicstyle=\ttfamily\scriptsize]
 pair_less_VDMNat: () -> set of ((nat*nat) * (nat*nat))
@@ -590,8 +662,8 @@ lex_prod(ra,rb) ==
         mk_(a,a') in set ra or a = a' and mk_(b, b') in set rb };
 \end{vdmsl}
 %
-That is, the lexicographic product of possibilities that are ordered in its parameters. 
-The translation process is the same as above and produces\<close>
+That is, the lexicographic product of possibilities that are ordered in its
+parameters. The translation process is the same as above and produces\<close>
 
 definition pre_ack :: \<open>VDMNat \<Rightarrow> VDMNat \<Rightarrow> \<bool>\<close> where
   \<open>pre_ack m n \<equiv> inv_VDMNat m \<and> inv_VDMNat n\<close>
@@ -615,11 +687,11 @@ termination \<^marker>\<open>tag invisible\<close>
    apply (simp add: inv_VDMNat_def pre_ack_def)
   by (simp add: inv_VDMNat_def pair_less_VDMNat_def pre_ack_def)
 
-text \<open>The proofs are also similar, despite the more complex measure, because of
-available Isabelle automation. We also show that this version of Ackermann with
- \<^typ>\<open>VDMNat\<close> is equivalent to the usual Isabelle definition using \<^typ>\<open>\<nat>\<close>. 
-We omit details here, but have proved that they are equivalent by induction\<close>
-
+text \<open>The proofs are also similar, despite the more complex measure, because
+of available Isabelle automation. We also show that this version of Ackermann
+with \<^typ>\<open>VDMNat\<close> is equivalent to the usual Isabelle definition using
+\<^typ>\<open>\<nat>\<close>. We omit details here, but have proved that they are equivalent by
+induction\<close>
 (*<*)
 fun ack' :: \<open>\<nat> \<Rightarrow> \<nat> \<Rightarrow> \<nat>\<close> where
   "ack' 0 n             = Suc n"
@@ -627,7 +699,8 @@ fun ack' :: \<open>\<nat> \<Rightarrow> \<nat> \<Rightarrow> \<nat>\<close> wher
 | "ack' (Suc m) (Suc n) = ack' m (ack' (Suc m) n)"
 
 fun ack'' :: \<open>\<nat> \<Rightarrow> \<nat> \<Rightarrow> \<nat>\<close> where
-  \<open>ack'' m n = (if m = 0 then Suc n else if n = 0 then ack'' (m - 1) 1 else ack'' (m-1) (ack'' m (n -1)))\<close>
+  \<open>ack'' m n = (if m = 0 then Suc n else if n = 0 then 
+                  ack'' (m - 1) 1 else ack'' (m-1) (ack'' m (n -1)))\<close>
 lemma l_ack''_1[simp]: \<open>ack'' 0 n = Suc n\<close> by simp
 lemma l_ack''_2[simp]: \<open>ack'' (Suc m) 0 = ack'' m 1\<close> by simp
 lemma l_ack''_3[simp]: \<open>ack'' (Suc m) (Suc n) = ack'' m (ack'' (Suc m) n)\<close> by simp
@@ -638,7 +711,8 @@ function ack''' :: "\<nat> \<Rightarrow> \<nat> \<Rightarrow> \<nat>" where
 | "ack''' (Suc m) (Suc n) = ack''' m (ack''' (Suc m) n)"
   by (pat_completeness, auto) 
 termination 
-  text \<open>Through the sledgehammer version, I unpicked the various bits and pieces needed.\<close>
+  text \<open>Through the sledgehammer version, I unpicked the various bits and
+  pieces needed.\<close>
 (*
   using "termination" lessI pair_lessI1 pair_less_iff1 wf_pair_less by presburger
 *)
@@ -653,17 +727,18 @@ termination
 theorem ack_correct: \<open>ack' m n = ack m n\<close>
   apply (induction \<open>m\<close> \<open>n\<close> rule: ack'.induct) by (simp add: pre_ack_defs)+
 
-text \<open>In general, each complex recursion function will require such a setup. Fortunately, 
-Isabelle has a number of options available. Yet, in general, the more complex the recursion, 
-the more users will have to provide further automation.\<close>
+text \<open>In general, each complex recursion function will require such a setup.
+Fortunately, Isabelle has a number of options available. Yet, in general, the
+more complex the recursion, the more users will have to provide further
+automation.\<close>
 
 (**************************************************************************************************)
 subsection \<open>Harder examples\label{subsec:Hard}\<close>
 
 (*<*)
 
-text \<open>Other examples from @{cite SCT_POPL}. 
-Example 3 is Ackermann, example 4 is permutation. Example 5 are yet to be finished.\<close>
+text \<open>Other examples from @{cite SCT_POPL}. Example 3 is Ackermann, example 4
+is permutation. Example 5 are yet to be finished.\<close>
 
 fun sct1_rev :: \<open>'a list \<Rightarrow> 'a list\<close>
 and sct1_r1  :: \<open>'a list \<Rightarrow> 'a list \<Rightarrow> 'a list\<close> 
@@ -711,11 +786,11 @@ where
 
 (*>*)
 
-text \<open>The next examples are require an elaborate setup. We can handle all examples 
-from~@{cite SCT_POPL}. For example, the permutation function 
-shows permuting decreasing parameters with an involved measure. The precondition 
-was required for finishing the termination proof and shows an example why proofs over \<^typ>\<open>\<int>\<close>
-can be harder.  
+text \<open>The next examples are require an elaborate setup. We can handle all
+examples from~@{cite SCT_POPL}. For example, the permutation function shows
+permuting decreasing parameters with an involved measure. The precondition was
+required for finishing the termination proof and shows an example why proofs
+over \<^typ>\<open>\<int>\<close> can be harder.
 %
 \begin{vdmsl}[frame=none,basicstyle=\ttfamily\scriptsize]
     perm: int * int * int -> int 
@@ -751,10 +826,10 @@ definition \<open>perm_wf_rel \<equiv>
    { ((m, r-1, n), (m, n, r)) | m r n . pre_perm m n r \<and> 0 < r } \<union> 
    { ((r, n-1, m), (m, n, r)) | m r n . pre_perm m n r \<and> \<not> 0 < r \<and> 0 < n }\<close>
 
-text \<open>Its measure relation contains elements for each recursive call, 
-filtered for the corresponding if-then case. The proof of well-formedness of 
-such measure relations involving multiple recursive calls require further 
-proof engineering, which is stated with the next lemma.\<close> 
+text \<open>Its measure relation contains elements for each recursive call, filtered
+for the corresponding if-then case. The proof of well-formedness of such
+measure relations involving multiple recursive calls require further proof
+engineering, which is stated with the next lemma.\<close>
 
 lemma l_perm_wf_rel_VDM_measure: 
   \<open>perm_wf_rel \<subseteq> measure (\<lambda> (m, r, n) . nat (max 0 (m+r+n)))\<close>
@@ -767,11 +842,12 @@ proof - \<^marker>\<open>tag invisible\<close>
     done
 qed
 
-text \<open>The Isabelle \<^term>\<open>measure\<close> function projects the inverse 
-image\<^footnote>\<open>Inverse image is defined as @{term[display] inv_image} or @{thm inv_image_def}.\<close> 
-of a given function as the recursive measure relation. Here the VDM-defined measure
-is given as such measure function projection. This highlights to the VDM user 
-the relationship (and differences) between VDM and Isabelle recursive measures.\<close>
+text \<open>The Isabelle \<^term>\<open>measure\<close> function projects the inverse
+image\<^footnote>\<open>Inverse image is defined as @{term[display] inv_image} or @{thm
+inv_image_def}.\<close> of a given function as the recursive measure relation. Here
+the VDM-defined measure is given as such measure function projection. This
+highlights to the VDM user the relationship (and differences) between VDM and
+Isabelle recursive measures.\<close>
 
 lemma l_perm_wf_rel: "wf perm_wf_rel" 
 proof - \<^marker>\<open>tag invisible\<close>
@@ -779,10 +855,10 @@ proof - \<^marker>\<open>tag invisible\<close>
   by (rule wf_subset [OF wf_measure])
 qed
 
-text \<open>This enables us to establish @{term perm_wf_rel} is well formed. The setup
-works here if the @{term pre_perm} specifically curbs negative sums of parameters. 
-This was not immediately obvious. With the added precondition the termination proof 
-is discovered by @{command sledgehammer}.\<close>
+text \<open>This enables us to establish @{term perm_wf_rel} is well formed. The
+setup works here if the @{term pre_perm} specifically curbs negative sums of
+parameters. This was not immediately obvious. With the added precondition the
+termination proof is discovered by @{command sledgehammer}.\<close>
 termination \<^marker>\<open>tag invisible\<close>
   apply (relation \<open>perm_wf_rel\<close>)
     apply (simp add: l_perm_wf_rel)
@@ -790,32 +866,31 @@ termination \<^marker>\<open>tag invisible\<close>
   done
 
 
-text \<open>Finally, the Takeuchi's 
-function\<^footnote>\<open>\<^url>\<open>https://isabelle.in.tum.de/library/HOL/HOL-Examples/Functions.html\<close>\<close>, 
-which contains both permutation and inner recursion is defined next, 
-where the important part is the SCNP setup using multi-sets @{cite KrausSCNP}, 
-given that ordered lexicographic products are not 
-strong enough to capture this type of recursion. It has not implicit precondition.
-The translation strategy works for these definitions, yet stands little chance 
-of finding proofs automatically.\<close>
-
+text \<open>Finally, the Takeuchi's
+function\<^footnote>\<open>\<^url>\<open>https://isabelle.in.tum.de/library/HOL/HOL-Examples/Functions.html\<close>\<close>,
+which contains both permutation and inner recursion is defined next, where the
+important part is the SCNP setup using multi-sets @{cite KrausSCNP}, given
+that ordered lexicographic products are not strong enough to capture this type
+of recursion. It has not implicit precondition. The translation strategy works
+for these definitions, yet stands little chance of finding proofs
+automatically.\<close>
 function (domintros) tak :: "VDMInt \<Rightarrow> VDMInt \<Rightarrow> VDMInt \<Rightarrow> VDMInt" where
   "tak x y z = (if x \<le> y then y else tak (tak (x-1) y z) (tak (y-1) z x) (tak (z-1) x y))"
   by auto
 
-(*<*)
-text \<open>Example of how one has to keep domain predicates as assumptions prior to termination proof.\<close>
+text \<open>Next is an example of how one has to keep domain predicates as 
+assumptions prior to termination proofs.\<close>
 lemma tak_pcorrect:
   "tak_dom (x, y, z) \<Longrightarrow> tak x y z = (if x \<le> y then y else if y \<le> z then z else x)"
-  thm tak.pinduct tak.psimps
-  apply (induction x y z rule: tak.pinduct) 
-  by (simp add: tak.psimps)
-(*>*)
+  thm tak.pinduct tak.psimps \<^marker>\<open>tag invisible\<close>
+  apply (induction x y z rule: tak.pinduct) \<^marker>\<open>tag invisible\<close>
+  by (simp add: tak.psimps) \<^marker>\<open>tag invisible\<close>
 
-text \<open>Each case (including non-recursive call) is represented in the SCNP setup, and then
-their measure-lexicographic\<^footnote>\<open>The measure-lexicographic product is represented as the 
-inverse image of the lexicographic product defined as @{thm mlex_prod_def}.\<close> 
-composition is used as the measure relation for the termination proof.\<close>
+text \<open>Each case (including non-recursive call) is represented in the SCNP
+setup, and then their measure-lexicographic\<^footnote>\<open>The measure-lexicographic product
+is represented as the inverse image of the lexicographic product defined as
+@{thm mlex_prod_def}.\<close> composition is used as the measure relation for the
+termination proof.\<close>
 definition tak_m1 where "tak_m1 = (\<lambda>(x,y,z). if x \<le> y then 0 else 1)"
 definition tak_m2 where "tak_m2 = (\<lambda>(x,y,z). nat (Max {x, y, z} - Min {x, y, z}))"
 definition tak_m3 where "tak_m3 = (\<lambda>(x,y,z). nat (x - Min {x, y, z}))"
@@ -865,8 +940,9 @@ lemma l_call4:
   by (simp add: case_prod_beta)
 (*>*)
 
-text \<open>The termination proof uses the measure relation @{term \<open>tak_m1 <*mlex*> tak_m2 <*mlex*> tak_m3 <*mlex*> {}\<close>}.
-  It requires user-defined lemmas for each of the four cases.\<close>
+text \<open>The termination proof uses the measure relation @{term \<open>tak_m1 <*mlex*>
+tak_m2 <*mlex*> tak_m3 <*mlex*> {}\<close>}. It requires user-defined lemmas for each
+of the four cases.\<close>
 termination \<^marker>\<open>tag invisible\<close>
   apply (relation "tak_m1 <*mlex*> tak_m2 <*mlex*> tak_m3 <*mlex*> {}") 
       apply (simp add: wf_mlex) 
@@ -875,19 +951,21 @@ termination \<^marker>\<open>tag invisible\<close>
      apply (simp add: l_call3)
   by (simp add: l_call4)
 
-text \<open>After the termination proof, the total version of induction and simplification 
-rules are available. Then, it is possible to prove its rather simpler equivalence.\<close>
+text \<open>After the termination proof, the total version of induction and
+simplification rules are available. Then, it is possible to prove its rather
+simpler equivalence.\<close>
 
 theorem tak_correct: "tak x y z = (if x \<le> y then y else if y \<le> z then z else x)"
   by (induction x y z rule: tak.induct) auto
 
-text \<open>Finally, we also want to tackle mutual recursion. VDM little bounds to mutually recursive
-definitions. Their proof obligations refer to each others measure functions. Isabelle requires
-all related definitions to be given in a single definition, where Isabelle's 
-sum (or union) types are used in the proof setup. Users have to annotate at least one of
-the mutually recursive definitions with \<^verbatim>\<open>@IsaMutualRec\<close> listing all function names involved.  
-Where needed, termination proof setup will be involved 
-and with limited automation. Here is a simple example and its translation.
+text \<open>Finally, we also want to tackle mutual recursion. VDM little bounds to
+mutually recursive definitions. Their proof obligations refer to each others
+measure functions. Isabelle requires all related definitions to be given in a
+single definition, where Isabelle's sum (or union) types are used in the proof
+setup. Users have to annotate at least one of the mutually recursive
+definitions with \<^verbatim>\<open>@IsaMutualRec\<close> listing all function names involved. Where
+needed, termination proof setup will be involved and with limited automation.
+Here is a simple example and its translation.
 %
 \begin{vdmsl}[frame=none,basicstyle=\ttfamily\scriptsize]
     --@IsaMutualRec({odd})
@@ -901,27 +979,28 @@ and with limited automation. Here is a simple example and its translation.
 \<close>
 definition pre_even :: \<open>VDMNat \<Rightarrow> \<bool>\<close> where [simp]: \<open>pre_even n \<equiv> inv_VDMNat n\<close> 
 definition pre_odd  :: \<open>VDMNat \<Rightarrow> \<bool>\<close> where [simp]: \<open>pre_odd n \<equiv> inv_VDMNat n\<close> 
-fun even :: \<open>VDMNat \<Rightarrow> \<bool>\<close> and odd  :: \<open>VDMNat \<Rightarrow> \<bool>\<close> where 
+fun (domintros) even :: \<open>VDMNat \<Rightarrow> \<bool>\<close> and odd  :: \<open>VDMNat \<Rightarrow> \<bool>\<close> where 
   \<open>even n = (if pre_even n then (if n = 0 then True else odd (n-1)) else undefined)\<close>
 | \<open>odd  n = (if pre_odd n then (if n = 0 then False else even (n-1)) else undefined)\<close>
 
 (**************************************************************************************************)
 section \<open>Discussion and conclusion\label{sec:Conclusion}\<close>
 
-text \<open>In this paper we present a translation strategy from VDM to Isabelle
-for recursive function over basic types, sets and maps. We also present how 
-the strategy works for more complex recursion, such as the Ackermann's function.
+text \<open>In this paper we present a translation strategy from VDM to Isabelle for
+recursive function over basic types, sets and maps. We also present how the
+strategy works for more complex recursion, such as the Ackermann's function.
 
-The complex recursion example also hints at possible VDM recursive measure extension
-to use a combination of measure relations and functions. The full VDM and Isabelle 
-sources and proofs can be found at the VDM toolkit repository 
+The complex recursion example also hints at possible VDM recursive measure
+extension to use a combination of measure relations and functions. The full
+VDM and Isabelle sources and proofs can be found at the VDM toolkit repository
 at \<^verbatim>\<open>RecursiveVDM*.thy\<close>\<^footnote>\<open>\<^url>\<open>https://github.com/leouk/VDM_Toolkit\<close>\<close>.\<close>
 
-paragraph \<open>Future work.~We are implementing the translation strategy in the \<^verbatim>\<open>vdm2isa\<close> plugin,
-which should be available soon. It is possible to discover all names within mutually 
-recursive calls. This will be useful to avoid having to write \<^verbatim>\<open>@IsaMutualRec\<close> annotations.\<close>
+paragraph \<open>Future work.~We are implementing the translation strategy in the
+\<^verbatim>\<open>vdm2isa\<close> plugin, which should be available soon. It is possible to discover
+all names within mutually recursive calls. This will be useful to avoid having
+to write \<^verbatim>\<open>@IsaMutualRec\<close> annotations.\<close>
 
-paragraph \<open>Acknowledgements.~We appreciated discussions with Stephan Merz on 
+paragraph \<open>Acknowledgements.~We appreciated discussions with Stephan Merz on
 pointers for complex well-founded recursion proofs in Isabelle, and with Nick
 Battle on limits for VDM recursive measures.\<close>
 
@@ -931,9 +1010,9 @@ lemma l_sumset_rel_wf': \<open>wf sumset_wf_rel\<close>
   apply (simp add: measure_def inv_image_def less_than_def less_eq)\<^marker>\<open>tag invisible\<close>
   apply (rule subsetI, simp add: case_prod_beta)\<^marker>\<open>tag invisible\<close>
   apply (elim exE conjE)\<^marker>\<open>tag invisible\<close>
-  by (metis card_Diff1_less_iff fst_conv inv_Map_defs(2) inv_Map_defs(3) pre_sumset_defs(1) snd_conv some_in_eq)\<^marker>\<open>tag invisible\<close>
+  by (metis card_Diff1_less_iff fst_conv inv_Map_defs(2) inv_Map_defs(3) 
+        pre_sumset_defs(1) snd_conv some_in_eq)\<^marker>\<open>tag invisible\<close>
 (*>*)
-
 
 (*<*)
 end
